theories/locks/invariant.v
@@ -1,0 +1,551 @@
+From diris.locks Require Export rtypesystem.
+From diris.locks Require Export definitions.
+
+Definition lock_rel (refcnt : nat) (o : option val) (ls : list lockcap) : Prop.
+Admitted.
+
+Definition lock_relM (refcnt : nat) (o : option val) (t : type) (in_l : multiset labelO) : Prop :=
+  ∃ lcs, in_l ≡ MultiSet (map (λ lc, LockLabel lc t) lcs) ∧ lock_rel refcnt o lcs.
+
+Global Instance lock_relM_Proper refcnt o t : Proper ((≡) ==> (≡)) (lock_relM refcnt o t).
+Proof.
+Admitted.
+
+Lemma lock_relM_newlock v t :
+  lock_relM 0 (Some v) t {[LockLabel (Owner, Closed) t]}.
+Proof.
+Admitted.
+
+Definition linv (ρ : cfg) (v : nat) (in_l : multiset labelO) : rProp :=
+  match ρ !! v with
+  | Some (Thread e) => ⌜⌜ in_l ≡ ε ⌝⌝ ∗ rtyped0 e UnitT
+  | Some Barrier => ⌜⌜ ∃ t1 t2 : type,
+      in_l ≡ {[ BarrierLabel false t1 t2 ]} ⋅
+             {[ BarrierLabel false t2 t1 ]} ⌝⌝
+  | Some (Lock refcnt o) => ∃ t,
+      ⌜⌜ lock_relM refcnt o t in_l ⌝⌝ ∗
+      match o with
+      | Some v => vtyped v t
+      | None => emp
+      end
+      (* Precisely one owner and k clients *)
+      (* if o is Some then one Opened and rest Closed,
+         if o is None then all Closed *)
+  | None => ⌜⌜ in_l ≡ ε ⌝⌝
+  end%I.
+
+Global Instance lin_Proper ρ v : Proper ((≡) ==> (≡)) (linv ρ v).
+Proof. solve_proper. Qed.
+
+Definition ginv ρ := inv (linv ρ).
+
+Lemma lookup_union_spec `{Countable K} {V} (m1 m2 : gmap K V) (x : K) :
+  (m1 ∪ m2) !! x = from_option Some (m2 !! x) (m1 !! x).
+Proof.
+  rewrite lookup_union.
+  destruct (m1 !! x),(m2 !! x); simpl; eauto.
+Qed.
+
+Ltac sdec := repeat (progress simp || case_decide || done || eauto).
+Ltac smap := repeat (
+  rewrite lookup_union_spec ||
+  rewrite lookup_alter_spec ||
+  rewrite lookup_insert_spec ||
+  rewrite lookup_delete_spec ||
+  rewrite lookup_empty || sdec).
+
+
+Lemma preservation i ρ ρ' :
+  step i ρ ρ' -> ginv ρ -> ginv ρ'.
+Proof.
+  intros H Hinv.
+  destruct H as [ρ ρ' ρf D1 D2 i H].
+  destruct H.
+  - eapply inv_impl; last done.
+    iIntros (n x) "H". unfold linv. smap.
+    iDestruct "H" as "[? H]". iFrame.
+    iDestruct (replacement with "H") as (t) "[H Q]"; first done.
+    iApply "Q". iApply pure_preservation; done.
+  - eapply inv_impl; last done.
+    iIntros (n x) "H". unfold linv. smap; iDestr "H";
+    assert (ρf !! n = None) as -> by solve_map_disjoint; eauto.
+    destruct v; simpl; iDestr "H"; simp. done.
+  - eapply (inv_alloc_lr i0 n j);
+    last done; first apply _; first apply _.
+    + naive_solver.
+    + iIntros (? ? ?) "H". unfold linv. smap.
+    + iIntros (?) "H". unfold linv. smap.
+      assert (ρf !! n = None) as -> by solve_map_disjoint; eauto.
+    + iIntros (?) "H". unfold linv. smap.
+      assert (ρf !! j = None) as -> by solve_map_disjoint; eauto.
+    + iIntros (?) "H". unfold linv. smap. iDestr "H".
+      iDestruct (replacement with "H") as (t) "[H Q]"; first done. simpl.
+      iDestr "H". simp.
+      iExists (BarrierLabel false t1 t2), (BarrierLabel false t2 t1).
+      iSplitL "Q".
+      * iIntros "H". iSplit; first done.
+        iApply "Q". simpl. eauto.
+      * iSplit; eauto.
+        iIntros "Q". iSplit; eauto 10 with iFrame.
+  - assert (inv (λ k x,
+      if decide (k = i0) then
+        ⌜⌜ x ≡ ε ⌝⌝ ∗ ∃ t1 t2, own_out n (BarrierLabel true t1 t2) ∗ ∀ e' : expr, rtyped0 e' t2 -∗ rtyped0 (k1 e') UnitT
+      else if decide (k = n) then
+        ∃ t1 t2, ⌜⌜ x ≡ {[ BarrierLabel true t1 t2 ]} ⋅ {[ BarrierLabel false t2 t1 ]} ⌝⌝ ∗
+        vtyped v1 t1
+      else if decide (k = j) then
+        ⌜⌜ x ≡ ε ⌝⌝ ∗ rtyped0 (k2 (App (Val (BarrierV n)) (Val v2))) UnitT
+      else linv ρf k x
+        )%I) as Hinv'.
+    {
+      eapply (inv_exchange i0 n); last done; [solve_proper|solve_proper|..].
+      - simp. smap; unfold linv; smap.
+      - simp. smap. unfold linv. smap.
+        iIntros "[% H]".
+        rewrite replacement; last done.
+        iDestruct "H" as (t1) "[H1 H2]". simpl.
+        iDestruct "H1" as (t2 l) "[H1 H3]".
+        iDestruct "H1" as (t1' t2' ?) "H1". simplify_eq.
+        iExists _. iFrame. iIntros (x [t1 [t2 ?]]) "".
+        eapply multiset_xsplit_singleton in H8 as [[]|[]]; simplify_eq.
+        + iExists _. iSplitL "H2".
+          * iIntros "H". iSplit; eauto. iExists _,_. iFrame.
+          * iExists _,_. iFrame. setoid_subst. eauto.
+        + iExists _. iSplitL "H2".
+          * iIntros "H". iSplit; eauto. iExists _,_. iFrame.
+          * iExists _,_. iFrame. setoid_subst. eauto.
+    } clear Hinv.
+
+    assert (inv (λ k x,
+      if decide (k = i0) then
+        ⌜⌜ x ≡ ε ⌝⌝ ∗ ∃ t1 t2, own_out n (BarrierLabel true t1 t2) ∗ ∀ e' : expr, rtyped0 e' t2 -∗ rtyped0 (k1 e') UnitT
+      else if decide (k = n) then
+        ∃ t1 t2, ⌜⌜ x ≡ {[ BarrierLabel true t1 t2 ]} ⌝⌝ ∗
+        vtyped v2 t2
+      else if decide (k = j) then
+        ⌜⌜ x ≡ ε ⌝⌝ ∗ rtyped0 (k2 (Val v1)) UnitT
+      else linv ρf k x
+        )%I) as Hinv''.
+    {
+      eapply (inv_dealloc j n); last done; [solve_proper|solve_proper|..].
+      - simp. smap.
+      - simp. smap.
+        iIntros "[% H]".
+        rewrite replacement; last done.
+        iDestruct "H" as (t1) "[H1 H2]". simpl.
+        iDestruct "H1" as (t2 l) "[H3 H4]".
+        iDestruct "H3" as (t1' t2' ?) "H". simplify_eq.
+        iExists _. iFrame. iIntros (?) "H".
+        iDestruct "H" as (t1 t2 ?) "H".
+        eapply multiset_xsplit_singleton in H8 as [[]|[]]; simplify_eq.
+        iSplitL "H H2".
+        + iSplit; eauto. iApply "H2". done.
+        + iExists _,_. iFrame. eauto.
+    } clear Hinv'.
+
+    eapply (inv_dealloc i0 n); last done; [solve_proper|solve_proper|..].
+    + simp. smap; unfold linv; smap.
+    + simp. smap.
+      iIntros "[% H]".
+      iDestruct "H" as (t1 t2) "[H1 H2]".
+      iExists _. iFrame. iIntros (?) "H".
+      iDestruct "H" as (t1' t2' ?) "H".
+      eapply multiset_singleton_mult' in H6 as []. simplify_eq.
+      unfold linv. smap.
+      assert (ρf !! n = None) as -> by solve_map_disjoint.
+      iSplit; eauto. iSplit; eauto.
+      iApply "H2". simpl. done.
+  - eapply (inv_alloc_l i0 n);
+    last done; first apply _; first apply _.
+    + done.
+    + iIntros (? ? ?) "H". unfold linv. smap.
+    + iIntros (?) "H". unfold linv. smap.
+      assert (ρf !! n = None) as -> by solve_map_disjoint; eauto.
+    + iIntros (?) "H". unfold linv. smap. iDestr "H".
+      iDestruct (replacement with "H") as (t) "[H Q]"; first done. simpl.
+      iDestr "H". simp.
+      iExists (LockLabel (Owner,Closed) t').
+      iSplitL "Q".
+      * iIntros "H". iSplit; first done.
+        iApply "Q". simpl. eauto.
+      * iExists t'. iFrame. iPureIntro. eapply lock_relM_newlock.
+  - eapply (inv_exchange_alloc i0 n j); last done; first apply _; first apply _.
+    + done.
+    + iIntros (? ? ?) "H". unfold linv. smap.
+    + iIntros (?) "H". unfold linv. smap.
+      assert (ρf !! j = None) as -> by solve_map_disjoint; eauto.
+    + iIntros (?) "H". unfold linv. smap. iDestr "H".
+      iDestruct (replacement with "H") as (t) "[H Q]"; first done. simpl.
+      iDestr "H". simp. iDestruct "H" as "[H1 H2]". iDestr "H1". simp.
+      iExists _. iFrame.
+      iIntros (?) "H". iDestr "H".
+      assert (t'0 = t) as -> by admit.
+      iExists (LockLabel l3 t),(LockLabel l2 t).
+      iSplitL "Q".
+      {
+        iIntros "H". iSplit; first done. iApply "Q". simpl.
+        iExists _,_. iSplit; done.
+      }
+      iSplitL "H".
+      * iExists _. iFrame. iPureIntro. admit.
+      * iIntros "H". eauto 10 with iFrame.
+  - eapply (inv_exchange i0 n);
+    last done; first apply _; first apply _.
+    + iIntros (? ? ?) "H". unfold linv. smap.
+    + iIntros (?) "H". unfold linv. smap. iDestr "H".
+      iDestruct (replacement with "H") as (t) "[H Q]"; first done. simpl.
+      iDestr "H". simp.
+      iExists _. iFrame. iIntros (x) "H". iDestr "H".
+      assert (t'0 = t) as -> by admit.
+      iExists (LockLabel _ _).
+      iSplitL "Q H".
+      * iIntros "H'". iSplit; first done.
+        iApply "Q". simpl. iExists _,_.
+        iSplit; first done. iFrame. iExists _,_. eauto.
+      * iExists t. iPureIntro. split; last done.
+        admit.
+  - eapply (inv_exchange i0 n);
+    last done; first apply _; first apply _.
+    + iIntros (? ? ?) "H". unfold linv. smap.
+    + iIntros (?) "H". unfold linv. smap. iDestr "H".
+      iDestruct (replacement with "H") as (t) "[H Q]"; first done. simpl.
+      iDestr "H". simp. iDestruct "H" as "[H1 H2]".
+      iDestr "H1". simp.
+      iExists _. iFrame. iIntros (x) "H". iDestr "H".
+      assert (t'0 = t) as -> by admit.
+      iExists (LockLabel _ _).
+      iSplitL "Q H".
+      * iIntros "H'". iSplit; first done.
+        iApply "Q". simpl. iExists _,_.
+        iSplit; first done. iFrame.
+      * iExists t. iFrame. iPureIntro.
+        admit.
+  - eapply (inv_dealloc i0 n);
+    last done; first apply _; first apply _.
+    + iIntros (? ? ?) "H". unfold linv. smap.
+    + iIntros (?) "H". unfold linv. smap. iDestr "H".
+      iDestruct (replacement with "H") as (t) "[H Q]"; first done. simpl.
+      iDestr "H". simp.
+      iExists _. iFrame. iIntros (x) "H". iDestr "H".
+      assert (t' = t) as -> by admit.
+      assert (ρf !! n = None) as -> by solve_map_disjoint.
+      iSplit; first iSplit; first done.
+      * iApply "Q". done.
+      * iPureIntro. admit.
+  - eapply (inv_dealloc i0 n);
+    last done; first apply _; first apply _.
+    + iIntros (? ? ?) "H". unfold linv. smap.
+    + iIntros (?) "H". unfold linv. smap. iDestr "H".
+      iDestruct (replacement with "H") as (t) "[H Q]"; first done. simpl.
+      iDestr "H". simp.
+      iExists _. iFrame. iIntros (x) "H". iDestr "H".
+      assert (t'0 = t) as -> by admit.
+      iSplitL "Q".
+      * iSplit; first done. iApply "Q". done.
+      * iExists _. iSplit; last done.
+        iPureIntro. admit.
+Admitted.
+
+Lemma fresh2 (s : gset nat) :
+  ∃ x y, x ∉ s ∧ y ∉ s ∧ x ≠ y.
+Proof.
+  exists (fresh s), (fresh (s ∪ {[ fresh s ]})).
+  split; first apply is_fresh.
+  pose proof (is_fresh (s ∪ {[ fresh s ]})).
+  set_solver.
+Qed.
+
+Lemma cfg_fresh2 (ρ : cfg) :
+  ∃ j1 j2, ρ !! j1 = None ∧ ρ !! j2 = None ∧ j1 ≠ j2.
+Proof.
+  destruct (fresh2 (dom ρ)) as (j1 & j2 & H1 & H2 & H3).
+  exists j1,j2. split_and!; last done;
+  apply not_elem_of_dom; done.
+Qed.
+
+Lemma linv_out_Some i j Σ l ρ x :
+  holds (linv ρ j x) Σ ->
+  Σ !! i ≡ Some l ->
+  ∃ e, ρ !! j = Some e.
+Proof.
+  unfold linv.
+  destruct (ρ !! j) as [[]|]; eauto.
+  rewrite affinely_pure_holds;
+  intros [H ?] Q; specialize (H i);
+  rewrite H lookup_empty in Q; simplify_eq.
+Qed.
+
+Definition own_dom A : rProp := ∃ Σ, ⌜⌜ A = dom Σ ⌝⌝ ∗ own Σ.
+
+Lemma own_dom_empty : own_dom ∅ ⊣⊢ emp.
+Proof.
+  iSplit; unfold own_dom; iIntros "H".
+  - iDestruct "H" as (? H) "H".
+    symmetry in H. apply dom_empty_iff_L in H as ->.
+    by iApply own_empty.
+  - iExists ∅. rewrite own_empty dom_empty_L //.
+Qed.
+
+Lemma own_dom_singleton k v : own {[ k := v ]} ⊢ own_dom {[ k ]}.
+Proof.
+  iIntros "H". iExists {[ k := v ]}.
+  rewrite dom_singleton_L. iFrame. done.
+Qed.
+
+Lemma own_dom_union A B : own_dom A ∗ own_dom B ⊢ own_dom (A ∪ B).
+Proof.
+  iIntros "[H1 H2]".
+  iDestruct "H1" as (Σ1 H1) "H1".
+  iDestruct "H2" as (Σ2 H2) "H2". subst.
+  iExists (Σ1 ∪ Σ2). rewrite dom_union_L. iSplit; eauto.
+  iApply own_union. iFrame.
+Qed.
+
+Lemma own_dom_fin_gset `{Countable A} n (g : fin n -> A) (f : A -> gset vertex) :
+  ([∗ set] p ∈ fin_gset n g, own_dom (f p)) -∗ own_dom (big_union (fin_gset n (f ∘ g))).
+Proof.
+  induction n.
+  - rewrite !fin_gset_0 big_union_empty big_sepS_empty own_dom_empty //.
+  - rewrite !fin_gset_S big_union_singleton_union.
+    destruct (decide (g 0%fin ∈ fin_gset n (λ i : fin n, g (FS i)))).
+    + rewrite subseteq_union_1_L; last rewrite singleton_subseteq_l //.
+      rewrite subseteq_union_1_L; first apply IHn.
+      eapply elem_of_fin_gset in e.
+      intros ??.
+      eapply elem_of_big_union.
+      destruct e. simpl in *.
+      rewrite -H1 in H0.
+      eexists. split; last done.
+      eapply elem_of_fin_gset. eauto.
+    + rewrite big_sepS_insert //.
+      iIntros "[H1 H2]".
+      iDestruct (IHn with "H2") as "H2".
+      iApply own_dom_union. iFrame.
+Qed.
+
+Lemma own_dom_fin_union n f :
+  ([∗ set] p ∈ all_fin n, own_dom (f p)) ⊢ own_dom (fin_union n f).
+Proof.
+  iApply own_dom_fin_gset.
+Qed.
+
+Lemma own_dom_all {A} (f : A -> gset vertex) :
+  (∀ i, own_dom (f i)) ⊢ ⌜ ∀ i j, f i = f j ⌝.
+Proof.
+  apply entails_holds.
+  intros Σ H.
+  rewrite pure_holds. intros.
+  rewrite ->forall_holds in H.
+  assert (∀ i, f i = dom Σ).
+  { intros k. specialize (H k).
+    eapply exists_holds in H as [].
+    eapply pure_sep_holds in H as [].
+    eapply own_holds in H0.
+    rewrite -H0 H //. }
+  rewrite !H0 //.
+Qed.
+
+Lemma own_dom_and A B :
+  own_dom A ∧ own_dom B ⊢ ⌜ A = B ⌝.
+Proof.
+  iIntros "H".
+  iAssert (∀ c:bool, own_dom (if c then A else B))%I with "[H]" as "H".
+  { iIntros ([]).
+    - by iDestruct "H" as "[H _]".
+    - by iDestruct "H" as "[_ H]". }
+  iDestruct (own_dom_all with "H") as %Q.
+  specialize (Q true false). simpl in *. eauto.
+Qed.
+
+Lemma fin_union_same `{Countable A} n (s : gset A) :
+  fin_union (S n) (λ i, s) = s.
+Proof.
+  induction n.
+  - rewrite fin_union_S fin_union_0 right_id_L //.
+  - rewrite fin_union_S IHn union_idemp_L //.
+Qed.
+
+Lemma rtyped_refs Γ e t :
+  rtyped Γ e t ⊢ own_dom (expr_refs e)
+with val_typed_refs v t :
+  vtyped v t ⊢ own_dom (val_refs v).
+Proof.
+  - iIntros "H". destruct e; simpl; repeat (iDestruct "H" as (?) "H"); try destruct l;
+    rewrite ?val_typed_refs ?rtyped_refs ?own_dom_empty ?own_dom_union; eauto.
+    iDestruct "H" as "[H1 H]". iApply own_dom_union; iFrame.
+    case_decide; subst. { rewrite fin_union_0 own_dom_empty //. }
+    setoid_rewrite rtyped_refs.
+    iDestruct (own_dom_all with "H") as %Q.
+    destruct n; simplify_eq.
+    assert (expr_refs ∘ e0 = λ i, expr_refs (e0 0%fin)) as ->.
+    { apply functional_extensionality. intros. eapply Q. }
+    rewrite fin_union_same. iApply "H".
+  - iIntros "H". destruct v; simpl; rewrite ?own_dom_empty; eauto;
+    repeat (iDestruct "H" as (?) "H"); try destruct l;
+    rewrite ?val_typed_refs ?rtyped_refs ?own_dom_union; eauto;
+    by iApply own_dom_singleton.
+Qed.
+
+Lemma expr_refs_linv ρ j e x Σ :
+  ρ !! j = Some (Thread e) ->
+  holds (linv ρ j x) Σ ->
+  expr_refs e = dom Σ.
+Proof.
+  intros H1 H2.
+  unfold linv in *.
+  rewrite H1 in H2.
+  eapply pure_sep_holds in H2 as [_ H2].
+  rewrite -rtyped_rtyped0 in H2.
+  eapply holds_entails in H2; last eapply rtyped_refs.
+  unfold own_dom in *.
+  eapply exists_holds in H2 as [Σ' H2].
+  eapply pure_sep_holds in H2 as [-> H2].
+  eapply own_holds in H2. rewrite H2 //.
+Qed.
+
+Lemma full_reachability ρ :
+  ginv ρ -> fully_reachable ρ.
+Proof.
+Admitted.
+  (* unfold fully_reachable.
+  intros Hinv.
+  destruct Hinv as [g [Hwf Hinv]].
+  eapply (cgraph_ind' (λ a b l, waiting ρ a b)); eauto; first solve_proper.
+  intros i IH1 IH2.
+  classical_right.
+  rewrite /inactive in H.
+  pose proof (Hinv i) as Q.
+  unfold linv in Q.
+  destruct (ρ !! i) eqn:E; simplify_eq. clear H.
+  destruct o.
+  - apply pure_sep_holds in Q as [Q1 Q2]. assert (Q2' := Q2).
+    eapply holds_entails in Q2; last apply pure_progress.
+    assert (ρ = {[ i := Thread e ]} ∪ delete i ρ) as HH.
+    { apply map_eq. intro. smap. } rewrite HH.
+    apply pure_holds in Q2 as [[v ->]|Q].
+    + constructor. exists (∅ ∪ delete i ρ).
+      econstructor; last constructor; last solve_map_disjoint.
+      intro x. smap. destruct (_!!x); done.
+    + destruct Q as (k & e0 & [Hk ->] & [[e0' Q] | [[v ->] | [v [j ->]]]]).
+      * constructor. eexists ({[ i := Thread (k e0') ]} ∪ delete i ρ).
+        constructor; [intro j; smap; by destruct (_!!j)..|].
+        constructor; eauto.
+      * constructor.
+        destruct (cfg_fresh2 ρ) as (j & n & Hj & Hn & Hjn).
+        exists ({[ i := Thread (k $ Val $ BarrierV n);
+                   j := Thread (App (Val v) (Val $ BarrierV n));
+                   n := Barrier ]} ∪ delete i ρ).
+        constructor; [intro x; smap; by destruct (_!!x)..|].
+        constructor; eauto; intros ->; simplify_eq.
+      * (* Thread is now trying to sync with a barrier *)
+        (* It is therefore waiting and reachable *)
+        rewrite -HH.
+        assert (∃ l, out_edges g i !! j ≡ Some l) as [l Hl].
+        {
+          (* rewrite replacement in Q2'; last done. *)
+          (* simpl in Q2'. *)
+          assert (holds ((∃ l, own_out j l) ∗ True) (out_edges g i)) as QQ.
+          {
+            eapply holds_entails; first exact Q2'.
+            iIntros "H".
+            rewrite replacement; last done.
+            iDestruct "H" as (t) "[H1 H2]".
+            simpl.
+            iDestruct "H1" as (t2 l) "[H11 H12]".
+            iDestruct "H11" as (t1 t0 ?) "H11". simplify_eq.
+            iSplitL "H11"; eauto.
+          }
+          eapply sep_holds in QQ as (Σ1 & Σ2 & H12 & Hdisj & Hout & HP).
+          eapply exists_holds in Hout as [l Hout].
+          unfold own_out in Hout.
+          eapply own_holds in Hout.
+          exists l. rewrite H12.
+          rewrite -Hout.
+          smap.
+        }
+        assert (ρ !! j = Some Barrier) as F.
+        {
+          eapply out_edges_in_labels in Hl as [x Hx].
+          specialize (Hinv j).
+          rewrite Hx in Hinv.
+          eapply pure_holds.
+          eapply holds_entails; first exact Hinv.
+          iIntros "H".
+          unfold linv.
+          destruct (ρ !! j) as [[]|]; eauto.
+          - iDestruct "H" as (?) "H".
+            exfalso. eapply multiset_empty_neq_singleton.
+            eapply multiset_empty_mult in H as []; eauto.
+          - iDestruct "H" as "%".
+            exfalso. eapply multiset_empty_neq_singleton.
+            eapply multiset_empty_mult in H as []; eauto.
+        }
+        assert (waiting ρ i j). {
+          unfold waiting. rewrite E F.
+          unfold expr_waiting; eauto.
+        }
+        assert (reachable ρ j). {
+          edestruct (IH1 j); eauto.
+          unfold inactive in *. simplify_eq.
+        }
+        eauto using reachable.
+  - eapply affinely_pure_holds in Q as [Q1 [t1 [t2 Q2]]].
+    (* Need to check whether both threads are trying to sync. *)
+    (* If so, then can_step *)
+    (* Otherwise, use IH *)
+    apply in_labels_out_edges2 in Q2 as (j1 & j2 & Hj12 & Hj1 & Hj2).
+
+    edestruct (linv_out_Some i j1) as [e1 He1]; eauto.
+    edestruct (linv_out_Some i j2) as [e2 He2]; eauto.
+
+    destruct (classic (waiting ρ j1 i)) as [W1|W1]; last first.
+    {
+      edestruct IH2; [|done|..]; eauto.
+      - unfold inactive in H. simplify_eq.
+      - assert (waiting ρ i j1); eauto using reachable.
+        unfold waiting in *.
+        rewrite He1 E in W1.
+        rewrite E He1. split; eauto.
+        erewrite expr_refs_linv; eauto.
+        apply elem_of_dom. rewrite Hj1. done.
+    }
+    destruct (classic (waiting ρ j2 i)) as [W2|W2]; last first.
+    {
+      edestruct IH2; [|done|..]; eauto.
+      - unfold inactive in H. simplify_eq.
+      - assert (waiting ρ i j2); eauto using reachable.
+        unfold waiting in *.
+        rewrite He2 E in W2.
+        rewrite E He2. split; eauto.
+        erewrite expr_refs_linv; eauto.
+        apply elem_of_dom. rewrite Hj2. done.
+    }
+    constructor.
+    unfold waiting in W1,W2.
+    rewrite He1 E in W1.
+    rewrite He2 E in W2.
+    assert (ρ = {[ j1 := Thread e1; j2 := Thread e2; i := Barrier ]} ∪ (delete j2 $ delete j1 $ delete i ρ)) as HH.
+    { apply map_eq. intro. smap. }
+    destruct W2 as (k2 & v2 & Hk2 & ->).
+    destruct W1 as (k1 & v1 & Hk1 & ->).
+    unfold can_step.
+    exists ({[ j1 := Thread (k1 $ Val v2); j2 := Thread (k2 $ Val v1) ]} ∪ (delete j2 $ delete j1 $ delete i ρ)).
+    rewrite {1}HH.
+    constructor.
+    { intro x. smap. destruct (_!!x); done. }
+    { intro x. smap. destruct (_!!x); done. }
+    constructor; eauto; intros ->; simplify_eq.
+Qed. *)
+
+Lemma initialization e :
+  typed ∅ e UnitT -> ginv {[ 0 := Thread e ]}.
+Proof.
+  intros H.
+  unfold ginv, linv.
+  eapply inv_impl; last eauto using inv_init.
+  intros. simpl.
+  iIntros "[% _]".
+  smap. iSplit; eauto.
+  rewrite -rtyped_rtyped0.
+  iApply typed_rtyped. eauto.
+Qed.
