theories/locks/langtools.v
@@ -1,0 +1,8 @@
+From iris.proofmode Require Export base tactics classes.
+From diris.cgraphs Require Export util.
+From Coq.Logic Require Export FunctionalExtensionality Classical.
+From diris Require Export seplogic.
+From stdpp Require Export gmap.
+Require Export diris.cgraphs.genericinv.
+
+Ltac inv H := inversion H; clear H; simplify_eq.
