theories/misc/tc.v
@@ -1,0 +1,89 @@
+From iris.proofmode Require Export base tactics classes.
+
+Lemma bar (P A : Prop) : ((P ∨ ¬ P) -> A) -> ¬ ¬ A.
+Proof.
+  intros H.
+  cut ((¬ ¬ (P ∨ ¬ P) -> ¬ ¬ A)).
+  - intros H2.
+    eapply H2. admit.
+  - intros H2 nA. eapply H2. intros Q.
+    eapply nA. eapply H. apply Q.
+Admitted.
+
+Lemma bar' (A : Prop) : ((∀ P, P ∨ ¬ P) -> A) -> ¬ ¬ A.
+Proof.
+  intros H.
+  cut (((∀ P, ¬ ¬ (P ∨ ¬ P)) -> ¬ ¬ A)).
+  - admit.
+  - intros H2 nA. eapply H2. intros Q.
+  eapply nA. eapply H. apply Q.
+Admitted.
+
+Lemma foo (A : Prop) : ((∀ P, P ∨ ¬ P) -> A) -> ¬ ¬ A.
+Proof.
+  intros H.
+  eapply (bar (∀ P, P ∨ ¬ P)).
+  intros L.
+  destruct L.
+  - eauto.
+  - intro. eapply H0.
+  Na.
+
+
+
+Axiom (A B C D : Prop).
+
+Axiom ab : A -> B.
+Axiom bc : B -> C.
+Axiom cc : C -> C.
+Axiom foo : (A -> C) -> D.
+
+Create HintDb X.
+Hint Resolve ab bc cc foo : X.
+
+Lemma bar : D.
+Proof.
+  debug eauto with X.
+Qed.
+
+Print bar.
+
+Class Y (p : Prop) := { inh : p }.
+
+Instance yab : Y A -> Y B.
+Proof.
+  intros []. constructor.
+  apply ab. assumption.
+Qed.
+
+Instance ybc : Y B -> Y C.
+Proof.
+  intros []. constructor.
+  apply bc. assumption.
+Qed.
+
+Instance yfoo : (Y A -> Y C) -> Y D.
+Proof.
+  intros H. constructor.
+  eapply foo. intro.
+  destruct H.
+  - constructor. assumption.
+  - assumption.
+Qed.
+
+Definition f : D := inh.
+
+Print f.
+
+Instance ybc
+
+Instance yab : Y A -> Y B :=
+  fun H : Y A =>
+  match H with
+  | {| inh := x |} => {| inh := ab x |}
+  end.
+
+Instance
+
+Print yab.
+  done.
